

BSE 666 Assignment 2

Q1] Taylor Series Approximation

$f(x) = x^4 - 3x^3 + 2x^2 + 7$, $x_0 = 2$ base point
estimate $f(3)$

Ans :

| | |
|--------------------------------|-------------------|
| $f(x) = x^4 - 3x^3 + 2x^2 + 7$ | $f(x_0=2) = 7$ |
| $f'(x) = 4x^3 - 9x^2 + 4x$ | $f'(x_0=2) = 4$ |
| $f''(x) = 12x^2 - 18x + 4$ | $f''(x_0=2) = 16$ |

Taylor expansion about $x_0 = 2$:

$$f(x) \approx f(2) + f'(2) \cdot (x-2) + \frac{f''(2)}{2!} (x-2)^2 \dots$$

0th order : $f(x) \approx f(2)$

1st order : $f(x) \approx f(2) + f'(2) \cdot (x-2)$

2nd order : $f(x) \approx f(2) + f'(2) \cdot (x-2) + \frac{f''(2)}{2!} (x-2)^2$

\therefore 0th order $f(3)$ estimate = $f(2) = 7$

1st order $f(3)$ estimate = $f(2) + f'(2) \cdot (1) = 11$

2nd order $f(3)$ estimate = $f(2) + f'(2) + \frac{f''(2)}{2} = 19$

exact $f(3) = 2.5$

| Approximation | $f(3)$ estimate | $f(3)$ exact | % error |
|---------------|-----------------|--------------|---------|
| zeroth | 7 | 2.5 | 72% |
| Linear | 11 | 2.5 | 56% |
| quadratic | 19 | 2.5 | 24% |

Derivative Approximations

0th order $f(x) \approx f(2) \therefore$ Derivative $f'(x) \approx 0$

1st order $f(x) \approx f(2) + f'(2) \cdot (x-2) \therefore$ Derivative $f'(x) \approx f'(2)$

2nd order $f(x) \approx f(2) + f'(2) \cdot (x-2) + \frac{f''(2)}{2!} (x-2)^2$
 \therefore Derivative $f'(x) \approx f'(2) + f''(2) \cdot (x-2)$

$$\text{exact } f'(3) = 4(3)^3 - 9(3)^2 + 4(3) = 39$$

| Approximation | $f'(3)$ estimate | exact $f'(3)$ | % error |
|---------------|-----------------------------------|---------------|---------|
| Zeroth | 0 | 39 | 100% |
| Linear | $f'(2) = 4$ | 39 | 89.7% |
| Quadratic | $f'(2) + f''(2) \cdot (3-2) = 20$ | 39 | 48.7% |

Q2] Newton Raphson method, initial (1, 1, 1), 4 iterations

$$f_1: x_1 - x_2 - x_3 = 0$$

$$f_2: 0 + x_2^2 - x_3^2 = 0$$

$$f_3: x_1^2 + x_2^2 + 2x_3^2 = 7$$

Ans: Let $\bar{x} = \begin{bmatrix} x_1 \\ x_2 \\ x_3 \end{bmatrix}$ $\bar{F}(\bar{x}) = \begin{bmatrix} f_1 \\ f_2 \\ f_3 \end{bmatrix}$

$$\text{Jacobian } \mathbb{J}(\bar{x}) = \frac{\partial \bar{F}}{\partial \bar{x}} = \begin{bmatrix} \frac{\partial f_1}{\partial x_1} & \frac{\partial f_1}{\partial x_2} & \frac{\partial f_1}{\partial x_3} \\ \frac{\partial f_2}{\partial x_1} & \frac{\partial f_2}{\partial x_2} & \frac{\partial f_2}{\partial x_3} \\ \frac{\partial f_3}{\partial x_1} & \frac{\partial f_3}{\partial x_2} & \frac{\partial f_3}{\partial x_3} \end{bmatrix} = \begin{bmatrix} 1 & -1 & -1 \\ 0 & 2x_2 & -2x_3 \\ 2x_1 & 2x_2 & 4x_3 \end{bmatrix}$$

$$\mathbb{J}(\bar{x}^{(k)}) \cdot \Delta \bar{x}^{(k)} = -\bar{F}(\bar{x}^{(k)}), \quad \bar{x}^{(k+1)} = \bar{x}^{(k)} - \Delta \bar{x}^{(k)}$$

0th iter: $\bar{x}^{(0)} = (1, 1, 1)$

$$\bar{F}(\bar{x}^{(0)}) = \begin{bmatrix} 1 - 1 - 1 \\ 0 + 1 - 1 \\ 1 + 1 + 2(1)^2 - 7 \end{bmatrix} = \begin{bmatrix} -1 \\ 0 \\ -3 \end{bmatrix} \quad \|\bar{F}\|_{\text{rms}} = \sqrt{\frac{f_1^2 + f_2^2 + f_3^2}{3}} = 1.825$$

$$\mathbb{J}(\bar{x}^{(0)}) = \begin{bmatrix} 1 & -1 & -1 \\ 0 & 2 & -2 \\ 2 & 2 & 4 \end{bmatrix}$$

$$\text{Solve } \mathbb{J} \cdot \Delta \bar{x} = -\bar{F}: \begin{bmatrix} 1 & -1 & -1 \\ 0 & 2 & -2 \\ 2 & 2 & 4 \end{bmatrix} \begin{bmatrix} \Delta x_1 \\ \Delta x_2 \\ \Delta x_3 \end{bmatrix} = \begin{bmatrix} -1 \\ 0 \\ -3 \end{bmatrix}$$

$$\text{get } \Delta \bar{x}^{(0)} = \begin{bmatrix} -1.2 \\ -0.1 \\ -0.1 \end{bmatrix} \quad \text{update } \bar{x}^{(1)} = \bar{x}^{(0)} - \Delta \bar{x}^{(0)} = \begin{bmatrix} 2.2 \\ 1.1 \\ 1.1 \end{bmatrix}$$

Iter (1) $x^{(1)} = \begin{bmatrix} 2.2 \\ 1.1 \\ 1.1 \end{bmatrix}$ $F(x^{(1)}) = \begin{bmatrix} 0 \\ 0 \\ 1.47 \end{bmatrix}$ $J(x^{(1)}) = \begin{bmatrix} 1 & -1 & -1 \\ 0 & 2.2 & -2.2 \\ 4.4 & 2.2 & 4.4 \end{bmatrix}$

Solve $J \Delta x^{(1)} = F$: $\begin{bmatrix} 1 & -1 & -1 \\ 0 & 2.2 & -2.2 \\ 4.4 & 2.2 & 4.4 \end{bmatrix} \begin{bmatrix} \Delta x_1^{(1)} \\ \Delta x_2^{(1)} \\ \Delta x_3^{(1)} \end{bmatrix} = \begin{bmatrix} 0 \\ 0 \\ 1.47 \end{bmatrix}$

get $\Delta x^{(1)} = \begin{bmatrix} 0.1909 \\ 0.0954 \\ 0.0954 \end{bmatrix}$ $\therefore x^{(2)} = x^{(1)} - \Delta x^{(1)}$
 $= \begin{bmatrix} 2.0090 \\ 1.0045 \\ 1.0045 \end{bmatrix}$

Iter (2) $x^{(2)} = \begin{bmatrix} 2.0090 \\ 1.0045 \\ 1.0045 \end{bmatrix}$ $F(x^{(2)}) = \begin{bmatrix} 0 \\ 0 \\ 0.0637 \end{bmatrix}$ $J(x^{(2)}) = \begin{bmatrix} 1 & -1 & -1 \\ 0 & 2.009 & -2.009 \\ 4.0181 & 2.009 & 4.0181 \end{bmatrix}$

$J \Delta x^{(2)} = F$ $\therefore \Delta x^{(2)} = \begin{bmatrix} 0.0090 \\ 0.0045 \\ 0.0045 \end{bmatrix}$

$x^{(3)} = x^{(2)} - \Delta x^{(2)} = \begin{bmatrix} 2.000 \\ 1.000 \\ 1.000 \end{bmatrix}$

[illegible]

| P | Q | R | S | T | U | V | W | X | Y | Z | AA | A |
|---|-----------------|----------|----------|---|----------|---|-----------------|----------|----------|---|------------------|---|
| | JACOBIAN iter 0 | | | | F iter0 | | J INVERSE iter0 | | | | dX=J.inv*F iter0 | |
| | 1 | -1 | -1 | | -1 | | 0.6 | 0.1 | 0.2 | | -1.2 | |
| | 0 | 2 | -2 | | 0 | | -0.2 | 0.3 | 0.1 | | -0.1 | |
| | 2 | 2 | 4 | | -3 | | -0.2 | -0.2 | 0.1 | | -0.1 | |
| | JACOBIAN ITER 1 | | | | F iter1 | | J INVERSE iter1 | | | | dX=J.inv*F iter1 | |
| | 1 | -1 | -1 | | 0 | | 0.428571 | 0.064935 | 0.12987 | | 0.190909091 | |
| | 0 | 2.2 | -2.2 | | 0 | | -0.28571 | 0.25974 | 0.064935 | | 0.095454545 | |
| | 4.4 | 2.2 | 4.4 | | 1.47 | | -0.28571 | -0.19481 | 0.064935 | | 0.095454545 | |
| | JACOBIAN ITER 2 | | | | F iter2 | | J INVERSE iter2 | | | | dX=J.inv*F iter2 | |
| | 1 | -1 | -1 | | 0 | | 0.428571 | 0.071105 | 0.142211 | | 0.009070341 | |
| | 0 | 2.009091 | -2.00909 | | 0 | | -0.28571 | 0.284421 | 0.071105 | | 0.004535171 | |
| | 4.018182 | 2.009091 | 4.018182 | | 0.063781 | | -0.28571 | -0.21332 | 0.071105 | | 0.004535171 | |
| | JACOBIAN ITER 3 | | | | F iter3 | | J INVERSE iter3 | | | | dX=J.inv*F iter3 | |
| | 1 | -1 | -1 | | 0 | | 0.428571 | 0.071428 | 0.142856 | | 2.05676E-05 | |
| | 0 | 2.000021 | -2.00002 | | 0 | | -0.28571 | 0.285711 | 0.071428 | | 1.02838E-05 | |
| | 4.000041 | 2.000021 | 4.000041 | | 0.000144 | | -0.28571 | -0.21428 | 0.071428 | | 1.02838E-05 | |

Q3] $\frac{d^2 T}{dx^2} - 2T^4 = 0$ $T(0) = 1$ $\frac{dT}{dx}(x=1) = 0$

5 equally spaced grid points on $0 \leq x \leq 1$

$x_1 = 0, x_2 = 0.25, x_3 = 0.5, x_4 = 0.75, x_5 = 1$

step $h = \frac{1-0}{5-1} = 0.25, \frac{1}{h^2} = 16$

unknown temperatures T_1, \dots, T_5

boundary conditions $T_1 = T(0) = 1$

neumann insulated tip $\left. \frac{dT}{dx} \right|_{x=1} = 0$

backward difference at $x_5 = 1: \frac{T_5 - T_4}{h} = 0$

$\therefore T_5 = T_4$

3 independent unknowns T_2, T_3, T_4

discretize ODE:

$\frac{T_{i+1} - 2T_i + T_{i-1}}{h^2} - 2T_i^4 = 0$ with $\frac{1}{h^2} = 16$

$i = \{2, 3, 4\}$

node 2: $16(T_3 - 2T_2 + T_1) - 2T_2^4 = 0$

node 3: $16(T_4 - 2T_3 + T_2) - 2T_3^4 = 0$

node 4: $16(T_5 - 2T_4 + T_3) - 2T_4^4 = 0$

but $T_5 = T_4 \therefore \Rightarrow 16(T_3 - T_4) - 2T_4^4 = 0$

non linear system

linearize (1st order TSA)

put $\rightarrow (T_i^{(k+1)})^4 \approx (T_i^{(k)})^4 + 4(T_i^{(k)})^3(T_i^{(k+1)} - T_i^{(k)})$ in T_i^4

node 2: $-16T_1 - 6(T_2^{(k)})^4$

node 3: $-6(T_3^{(k)})^4$

node 4: $-6(T_4^{(k)})^4$

For node i $\frac{T_{i+1} - 2T_i + T_{i-1}}{h^2} - 2T_i^4 = 0$

with $\frac{1}{h^2} = 16$

$$16(T_{i+1} - 2T_i + T_{i-1}) - 2T_i^4 = 0$$

non linear term
 $(T_i^{(k+1)})^4$

TSA 1st order:

$$\begin{aligned} (T_i^{(k+1)})^4 &\approx (T_i^{(k)})^4 + 4(T_i^{(k)})^3 (T_i^{(k+1)} - T_i^{(k)}) \\ &\approx 4(T_i^{(k)})^3 T_i^{(k+1)} - 3(T_i^{(k)})^4 \end{aligned}$$

plug : $-2(T_i^{(k+1)})^4 \approx -2(4(T_i^{(k)})^3 T_i^{(k+1)} - 3(T_i^{(k)})^4)$
 $= -8(T_i^{(k)})^3 T_i^{(k+1)} + 6(T_i^{(k)})^4$

$$\begin{aligned} \therefore 16 T_{i+1}^{(k+1)} - 32 T_i^{(k+1)} + 16 T_{i-1}^{(k+1)} - 8(T_i^{(k)})^3 T_i^{(k+1)} + 6(T_i^{(k)})^4 &= 0 \\ \therefore 16 T_{i+1}^{(k+1)} + 16 T_{i-1}^{(k+1)} + (-32 - 8(T_i^{(k)})^3) T_i^{(k+1)} &= -6(T_i^{(k)})^4 \end{aligned}$$

node 2: uses $T_1 = 1$ put $i = 2$

$$(-32 - 8(T_2^k)^3) T_2^{(k+1)} + 16 T_3^{(k+1)} = -16 T_1 - 6(T_2^k)^4$$

node 3 : $-6(T_3^k)^4$

node 4 : $-6(T_4^k)^4$

Matrix form: ~~A~~ $A^{(k)} \cdot T^{(k+1)} = b^{(k)}$

$$\text{let } T^{(k+1)} = \begin{bmatrix} T_2^{(k+1)} \\ T_3^{(k+1)} \\ T_4^{(k+1)} \end{bmatrix}$$

$$A^{(k)} = \begin{bmatrix} -32-8(T_2^k)^3 & 16 & 0 \\ 16 & -32-8(T_3^k)^3 & 16 \\ 0 & 16 & -16-8(T_4^k)^3 \end{bmatrix} \begin{bmatrix} T_2^{(k+1)} \\ T_3^{(k+1)} \\ T_4^{(k+1)} \end{bmatrix} = \begin{bmatrix} -16(T_1^k)^4 \\ -6(T_3^k)^4 \\ -6(T_4^k)^4 \end{bmatrix}$$

$\underbrace{\hspace{15em}}_{A^{(k)}} \quad \underbrace{\hspace{10em}}_{T^{(k+1)}} \quad \underbrace{\hspace{10em}}_{b^{(k)}}$

$T_1 = 1$ and $T_5^{(k+1)} = T_4^{(k+1)}$

initial: $T_1 = 1, T_2^{(0)} = 1 = T_3^{(0)} = T_4^{(0)} = T_5^{(0)}$

Q4) $h_1(t)$ $h_2(t)$ = water levels

A_1, A_2 = areas

$f_1(t)$ $f_2(t)$ = external inflows

$q_{12}(t)$ = tank 1 \rightarrow 2, $q_{20}(t)$ = tank 2 \rightarrow out

mass balance :

$$\therefore A_1 \frac{dh_1}{dt} = f_1(t) - q_{12}(t)$$

$$A_2 \frac{dh_2}{dt} = f_2(t) + q_{12}(t) - q_{20}(t)$$

tube flow model

$$q_{12} = C \cdot \sqrt{h_1 - h_2} \quad \text{with loss coefficient } C, h_1 \geq h_2$$

if $f_1 = f_2 = 0$ $q_{20} = 0$ $A_1 = A_2 = A$ then

$$A \frac{dh_1}{dt} = -q_{12} \quad A \frac{dh_2}{dt} = +q_{12} = C \cdot \sqrt{h_1 - h_2}$$

$$\therefore \text{coupled system : } \frac{dh_1}{dt} = -\frac{C}{A} \sqrt{h_1 - h_2}$$

$$\frac{dh_2}{dt} = \frac{C}{A} \sqrt{h_1 - h_2}$$

steady state $q_{12} = 0 \Rightarrow h_1 = h_2$

total volume conserved $\therefore (h_1 + h_2)$ constant

$$\therefore h_1(\infty) = h_2(\infty) = \frac{h_1 + h_2}{2}$$

let $t^n, t^{n+1} = t^n + \Delta t$

implicit: $h_1^{n+1} = h_1^n - \frac{\Delta t}{A} q_{12}^{n+1}$

$h_2^{n+1} = h_2^n + \frac{\Delta t}{A} q_{12}^{n+1}$

where $q_{12}^{n+1} = C \sqrt{h_1^{n+1} - h_2^{n+1}}$ — non linear

let $\alpha = \frac{\Delta t}{A}$ $\Delta h^{n+1} = h_1^{n+1} - h_2^{n+1}$

$\therefore h_1^{n+1} = h_1^n - \alpha C \sqrt{\Delta h^{n+1}}, h_2^{n+1} = h_2^n + \alpha C \sqrt{\Delta h^{n+1}}$

linearization about a guessed estimate 1st order TSA

$k = 0, 1, 2, \dots$

guess $(h_1^{n+1(k)}, h_2^{n+1(k)})$ $\Delta h^{(k)} = h_1^{n+1(k)} - h_2^{n+1(k)}$
 $q^{(k)} = C \sqrt{\Delta h^{(k)}}$

$\frac{dq}{d(\Delta h)} = \frac{C}{2\sqrt{\Delta h}}$

1st order TSA about $\Delta h^{(k)}$:

$q^{(k+1)} \approx q^{(k)} + d^{(k)} (\Delta h^{(k+1)} - \Delta h^{(k)})$

where $d^{(k)} \equiv \frac{C}{2\sqrt{\Delta h^{(k)}}}$

$q^{(k+1)}$
 plug into

$h_1^{n+1(k+1)} + \alpha q^{(k+1)} = h_1^n$
 $h_2^{n+1(k+1)} - \alpha q^{(k+1)} = h_2^n$

$$\begin{bmatrix} 1 + \alpha d^{(k)} & -\alpha d^{(k)} \\ -\alpha d^{(k)} & 1 + \alpha d^{(k)} \end{bmatrix} \begin{bmatrix} h_1^{n+1}(k+1) \\ h_2^{n+1}(k+1) \end{bmatrix} = \begin{bmatrix} h_1^n - \alpha g^{(k)} + \alpha d^{(k)} \Delta h^{(k)} \\ h_2^n + \alpha g^{(k)} - \alpha d^{(k)} \Delta h^{(k)} \end{bmatrix}$$

Algorithm

input h_1, h_2, A, C st final t_{\max} tolerance ϵ
 set $n=0$ $h_1^0 = h_1$ $h_2^0 = h_2$

for each $n \rightarrow n+1$ timestep
 $h_1^{n+1,0} = h_1^n$ $h_2^{n+1,0} = h_2^n$
 for $k=0, 1, 2, \dots$

$$\Delta h^{(k)} = h_1^{n+1}(k) - h_2^{n+1}(k)$$

$$g^{(k)} = C \sqrt{\Delta h^{(k)}}$$

$$d^{(k)} = \frac{C}{2\sqrt{\Delta h^{(k)}}}$$

solve for $h_1^{n+1}(k+1), h_2^{n+1}(k+1)$ using above matrix

$$\text{convergence check } \sqrt{(h_1^{k+1} - h_1^k)^2 + (h_2^{k+1} - h_2^k)^2} < \epsilon$$

set $h_1^{n+1} = h_1^{n+1}(k+1)$
 $t^{n+1} = t^n + \Delta t$

choose Δt : such that $\left\| \frac{h,^{n+1} - h,^n}{h,^n} \right\|$ is small